progress towards instantiating total heap state as a pcm

TotalStateUtil.thy
@@ -1,5 +1,5 @@
 theory TotalStateUtil
-imports TotalViperState Viper.DeBruijn
+imports Viper.SepAlgebra TotalViperState Viper.DeBruijn
 begin
 
 section \<open>update_store_total\<close>
@@ -12,7 +12,7 @@ fun update_store_total :: "'a full_total_state \<Rightarrow> 'a store \<Rightarr
 
 section \<open>update_trace_total\<close>
 
-fun update_trace_total :: "'a full_total_state \<Rightarrow> 'a total_trace \<Rightarrow> 'a full_total_state"
+fun update_trace_total :: "('a, 'b) full_total_state_scheme \<Rightarrow> 'a total_trace \<Rightarrow> ('a, 'b) full_total_state_scheme" 
   where "update_trace_total \<omega> \<pi> = \<omega>\<lparr>get_trace_total := \<pi>\<rparr>"
 
 lemma update_trace_total_store_same: "get_store_total (update_trace_total \<omega> \<pi>) = get_store_total \<omega>"
@@ -28,6 +28,12 @@ lemma update_trace_total_mask_same: "get_mh_total_full (update_trace_total \<ome
   by simp
 
 section \<open>heap and mask in total state\<close>
+
+fun get_m_total :: "('a, 'b) total_state_scheme \<Rightarrow> mask \<times> 'a predicate_mask"
+  where "get_m_total \<phi> = (get_mh_total \<phi>, get_mp_total \<phi>)"
+
+fun update_m_total :: "('a, 'b) total_state_scheme \<Rightarrow> mask \<times> 'a predicate_mask \<Rightarrow> ('a, 'b) total_state_scheme"
+  where "update_m_total \<phi> m = \<phi>\<lparr> get_mh_total := fst m, get_mp_total := snd m \<rparr>"
 
 fun update_hh_loc_total :: "'a total_state \<Rightarrow> heap_loc \<Rightarrow> 'a val \<Rightarrow> 'a total_state"
   where "update_hh_loc_total \<phi> l v = \<phi>\<lparr>get_hh_total := (get_hh_total \<phi>)(l := v)\<rparr>"
@@ -158,6 +164,270 @@ proof -
     apply (rule less_eq_full_total_stateI)
     by (fastforce dest: less_eq_full_total_stateD)+
 qed
+
+subsection \<open>Partial Commutative Monoid Instantiation\<close>
+
+lemma plus_masks_defined: "(m1 :: 'a abstract_mask) ## m2"
+  unfolding defined_def
+  by (simp add: SepAlgebra.plus_prat_def compatible_funI plus_fun_def)
+
+instantiation total_state_ext :: (type,type) pcm
+begin
+
+definition plus_total_state_ext :: "('a,'b) total_state_ext \<Rightarrow> ('a,'b) total_state_ext \<Rightarrow> ('a,'b) total_state_ext option"
+  where "plus_total_state_ext \<phi>1 \<phi>2 = 
+              (let (mh1, mp1, mh2, mp2) = (get_mh_total \<phi>1, get_mp_total \<phi>1, get_mh_total \<phi>2, get_mp_total \<phi>2) in 
+                   if get_hh_total \<phi>1 = get_hh_total \<phi>2 \<and> get_hp_total \<phi>1 = get_hp_total \<phi>2 \<and> 
+                      total_state.more \<phi>1 = total_state.more \<phi>2
+                   then Some (update_m_total \<phi>1 (the (mh1 \<oplus> mh2), the (mp1 \<oplus> mp2)))
+                   else None)"
+
+instance proof
+  fix a b ab c bc :: "('a,'b) total_state_ext"
+
+  let ?mh_a = "get_mh_total a"
+  let ?mp_a = "get_mp_total a"
+  let ?mh_b = "get_mh_total b"
+  let ?mp_b = "get_mp_total b"
+  let ?mh_c = "get_mh_total c"
+  let ?mp_c = "get_mp_total c"
+
+  obtain mh_ab where MhEqAB: "?mh_a \<oplus> ?mh_b = Some mh_ab" 
+    using plus_masks_defined
+    unfolding defined_def
+    by blast
+
+  obtain mp_ab where MpEqAB: "?mp_a \<oplus> ?mp_b = Some mp_ab"
+    using plus_masks_defined
+    unfolding defined_def
+    by blast
+
+  note MEqAB = MhEqAB MpEqAB
+
+  obtain mh_bc where MhEqBC: "?mh_b \<oplus> ?mh_c = Some mh_bc" 
+    using plus_masks_defined
+    unfolding defined_def
+    by blast
+
+  obtain mp_bc where MpEqBC: "?mp_b \<oplus> ?mp_c = Some mp_bc"
+    using plus_masks_defined
+    unfolding defined_def
+    by blast
+
+  note MEqBC = MhEqBC MpEqBC
+
+  show "a \<oplus> b = b \<oplus> a" 
+    unfolding plus_total_state_ext_def
+    by (simp add: commutative)      
+  
+  show "a \<oplus> b = Some ab \<and> b \<oplus> c = Some bc \<Longrightarrow> ab \<oplus> c = a \<oplus> bc"
+  proof -
+    have *: "mh_ab \<oplus> get_mh_total c = get_mh_total a \<oplus> mh_bc"
+      using MEqAB MEqBC asso1
+      by blast
+
+    have **: "mp_ab \<oplus> get_mp_total c = get_mp_total a \<oplus> mp_bc"
+      using MEqAB MEqBC asso1
+      by blast
+
+    assume "a \<oplus> b = Some ab \<and> b \<oplus> c = Some bc"
+    thus ?thesis
+    unfolding plus_total_state_ext_def
+    by (clarsimp simp: * ** MEqAB MEqBC split: if_split if_split_asm)
+  qed
+
+  show "a \<oplus> b = None \<and> b \<oplus> c = Some bc \<Longrightarrow> a \<oplus> bc = None"
+  unfolding plus_total_state_ext_def
+  by (clarsimp split: if_split if_split_asm)
+
+  show "a \<oplus> b = Some ab \<and> b \<oplus> c = None \<Longrightarrow> ab \<oplus> c = None"
+  unfolding plus_total_state_ext_def
+  by (clarsimp split: if_split if_split_asm)
+
+  show "a \<oplus> b = Some c \<Longrightarrow> Some c = c \<oplus> c \<Longrightarrow> Some a = a \<oplus> a"
+  proof -
+    assume A: "a \<oplus> b = Some c" and B: "Some c = c \<oplus> c"
+
+    obtain mh_cc where MhEqCC: "?mh_c \<oplus> ?mh_c = Some mh_cc"
+    using plus_masks_defined
+    unfolding defined_def
+    by blast
+
+    obtain mp_cc where MpEqCC: "?mp_c \<oplus> ?mp_c = Some mp_cc"
+    using plus_masks_defined
+    unfolding defined_def
+    by blast
+
+    note MEqCC = MhEqCC MpEqCC
+
+    from B have *: "?mh_c \<oplus> ?mh_c = Some ?mh_c \<and> ?mp_c \<oplus> ?mp_c = Some ?mp_c"
+      unfolding plus_total_state_ext_def
+      
+    proof (clarsimp simp: MEqCC split: if_split if_split_asm)
+      assume "c = c\<lparr>get_mh_total := mh_cc, get_mp_total := mp_cc\<rparr>"
+      have "get_mh_total c = mh_cc"
+        apply (subst \<open>c = _\<close>)
+        by simp
+      moreover have "get_mp_total c = mp_cc"
+        apply (subst \<open>c = _\<close>)
+        by simp
+      ultimately show "mh_cc = get_mh_total c \<and> mp_cc = get_mp_total c"
+        by simp
+    qed
+
+    moreover from * A have "?mh_a \<oplus> ?mh_b = Some ?mh_c \<and> ?mp_a \<oplus> ?mp_b = Some ?mp_c"
+      unfolding plus_total_state_ext_def
+      by (clarsimp simp: MEqAB split: if_split if_split_asm)
+
+    ultimately have "?mh_a \<oplus> ?mh_a = Some ?mh_a \<and> ?mp_a \<oplus> ?mp_a = Some ?mp_a"
+      using positivity
+      by metis
+
+    thus ?thesis
+      unfolding plus_total_state_ext_def
+      by (clarsimp simp: MEqAB MEqBC split: if_split if_split_asm)
+  qed    
+qed
+
+end
+
+instantiation full_total_state_ext :: (type,type) pcm
+begin
+
+definition plus_full_total_state_ext :: "('a,'b) full_total_state_ext \<Rightarrow> ('a,'b) full_total_state_ext \<Rightarrow> ('a,'b) full_total_state_ext option"
+  where "plus_full_total_state_ext \<omega>1 \<omega>2 = 
+            (if get_store_total \<omega>1 = get_store_total \<omega>2 \<and> 
+                get_trace_total \<omega>1 ## get_trace_total \<omega>2 \<and>
+                get_total_full \<omega>1 ## get_total_full \<omega>2 \<and>
+                full_total_state.more \<omega>1 = full_total_state.more \<omega>2 then
+                Some (\<omega>1\<lparr>get_trace_total := the (get_trace_total \<omega>1 \<oplus> get_trace_total \<omega>2),
+                         get_total_full := the (get_total_full \<omega>1 \<oplus> get_total_full \<omega>2) \<rparr>)
+            else 
+                undefined)"
+
+instance
+  sorry
+
+end
+
+term "core (a :: mask)"
+
+lemma plus_mask_zero_mask_neutral: "m \<oplus> zero_mask = Some m"
+proof -
+  have "compatible_fun m zero_mask"
+    by (simp add: SepAlgebra.plus_prat_def compatible_funI)
+
+  thus ?thesis
+  unfolding plus_fun_def
+  by (simp add: SepAlgebra.plus_prat_def zero_mask_def)
+qed
+
+lemma core_mask_zero_mask: "zero_mask = |m :: 'a abstract_mask|"
+proof 
+  fix x
+  show "zero_mask x = |m| x"
+    unfolding zero_mask_def
+    by (simp add: core_fun core_prat_def)
+qed
+
+lemma total_state_plus_defined: 
+  assumes "a \<oplus> b = Some c"
+  shows "get_hh_total a = get_hh_total b \<and> get_hp_total a = get_hp_total b \<and> total_state.more a = total_state.more b \<and>
+         get_hh_total a = get_hh_total c \<and> get_hp_total a = get_hp_total c \<and> total_state.more a = total_state.more c"
+  using assms
+  unfolding plus_total_state_ext_def
+  by (clarsimp split: if_split_asm ) 
+
+lemma mask_plus_Some:
+  shows "m1 \<oplus> m2 = Some (add_masks m1 m2)"
+  unfolding plus_fun_def add_masks_def
+  by (simp split: if_split add: SepAlgebra.plus_prat_def compatible_fun_def)
+
+lemma add_masks_self_zero_mask:
+  assumes "m1 = add_masks m1 m2"
+  shows "m2 = zero_mask"
+  using assms
+  unfolding add_masks_def
+  (* TODO: faster proof *)
+  by (metis add.commute add_0 le_fun_def order_class.order_eq_iff padd_cancellative zero_mask_def zero_mask_less_eq_mask)
+
+lemma plus_total_state_cancellative:
+  assumes "Some a = b \<oplus> x" and
+          "Some a = b \<oplus> y"
+        shows "x = y"
+  sorry
+
+instantiation total_state_ext :: (type,type) pcm_with_core
+begin
+
+definition core_total_state_ext :: "('a,'b) total_state_ext \<Rightarrow> ('a, 'b) total_state_ext"
+  where "core_total_state_ext \<phi> = (update_m_total \<phi> (zero_mask, zero_mask))"
+
+instance proof
+  fix a b c x y :: "('a,'b) total_state_ext"
+
+  show "Some x = x \<oplus> |x|"
+    unfolding core_total_state_ext_def plus_total_state_ext_def
+    apply simp
+    using plus_mask_zero_mask_neutral
+    by (metis option.sel total_state.surjective total_state.update_convs(3) total_state.update_convs(4))
     
+
+  show "Some |x| = |x| \<oplus> |x|"
+    unfolding core_total_state_ext_def plus_total_state_ext_def
+    apply simp
+    using plus_mask_zero_mask_neutral
+    by (metis option.sel)
+
+  show "Some x = x \<oplus> c \<Longrightarrow> \<exists>r. Some |x| = c \<oplus> r" (is "?lhs \<Longrightarrow> ?rhs")
+  proof -
+    assume ?lhs
+    hence "get_hh_total x = get_hh_total c \<and> get_hp_total x = get_hp_total c \<and> total_state.more x = total_state.more c"
+      unfolding plus_total_state_ext_def
+      by (smt (verit) case_prod_conv option.discI)
+
+    have *: "get_mh_total c = zero_mask \<and> get_mp_total c = zero_mask"
+    proof -
+      note MaskPlusEq = 
+          mask_plus_Some[of "get_mh_total x" "get_mh_total c"]
+          mask_plus_Some[of "get_mp_total x" "get_mp_total c"]
+
+      from \<open>?lhs\<close> show ?thesis
+        unfolding plus_total_state_ext_def
+        apply (simp split: if_split_asm)
+        apply (simp add: MaskPlusEq)
+        using add_masks_self_zero_mask
+        by (metis total_state.ext_inject total_state.surjective total_state.update_convs(3) total_state.update_convs(4))        
+    qed       
+
+    show ?thesis
+      unfolding core_total_state_ext_def plus_total_state_ext_def 
+     apply (rule exI[where ?x="c\<lparr> get_mh_total := zero_mask, get_mp_total := zero_mask \<rparr>"])
+     apply (simp add: * split: if_split if_split_asm)
+      apply (simp add: plus_mask_zero_mask_neutral[simplified commutative])
+      using total_state_plus_defined[OF HOL.sym[OF \<open>?lhs\<close>]]
+      by simp
+  qed
+
+  show "Some c = a \<oplus> b \<Longrightarrow> Some |c| = |a| \<oplus> |b|"
+    unfolding core_total_state_ext_def plus_total_state_ext_def
+    by (clarsimp split: if_split if_split_asm simp: plus_mask_zero_mask_neutral)
+
+  show "Some a = b \<oplus> x \<Longrightarrow> Some a = b \<oplus> y \<Longrightarrow> |x| = |y| \<Longrightarrow> x = y"
+    using plus_total_state_cancellative
+    by blast
+qed
+
+end
+
+instantiation full_total_state_ext :: (type,type) pcm_with_core
+begin
+
+definition full_core_total_state_ext :: "('a,'b) full_total_state_ext \<Rightarrow> ('a, 'b) full_total_state_ext"
+  where "full_core_total_state_ext \<phi> = 
+            \<phi> \<lparr> get_trace_total := |get_trace_total \<phi>|, get_total_full := |get_total_full \<phi>|\<rparr>"
+instance
+  sorry
+end
 
 end
